cleanup binary search

Test/CaseStudies/BinarySearch.lean
@@ -1,34 +1,40 @@
 import Chako
 
-
-@[specialize] def binSearchAux {α : Type u} {β : Type v} (lt : α → α → Bool) (found : Option α → β) (as : Array α) (k : α) :
-    (lo : Fin (as.size + 1)) → (hi : Fin as.size) → (lo.1 ≤ hi.1) → β
-  | lo, hi, h =>
-    let m := (lo.1 + hi.1)/2
-    let a := as[m]
-    if lt a k then
-      if h' : m + 1 ≤ hi.1 then
-        binSearchAux lt found as k ⟨m+1, by grind⟩ hi h'
-      else found none
-    else if lt k a then
-      if h' : m = 0 ∨ m - 1 < lo.1 then found none
-      else binSearchAux lt found as k lo ⟨m-1, by grind⟩ (by grind)
-    else found (some a)
-termination_by lo hi => hi.1 - lo.1
-
-@[inline] def binSearch {α : Type} (as : Array α) (k : α) (lt : α → α → Bool) (lo := 0) (hi := as.size - 1) : Option α :=
-  if h : lo < as.size then
-    let hi := if hi < as.size then hi else as.size - 1
-    if w : lo ≤ hi then
-      binSearchAux lt id as k ⟨lo, by grind⟩ ⟨hi, by grind⟩ (by grind)
+@[specialize]
+def binSearchAux {α : Type u} (lt : α → α → Bool) (as : Array α) (k : α) (lo : Fin (as.size + 1))
+    (hi : Fin as.size) (h : lo.1 ≤ hi.1) : Option α :=
+  let m := (lo.1 + hi.1) / 2
+  let a := as[m]
+  if lt a k then
+    if h' : m + 1 ≤ hi.1 then
+      binSearchAux lt as k ⟨m + 1, by grind⟩ hi h'
     else
       none
+  else if lt k a then
+    if h' : m = 0 ∨ m - 1 < lo.1 then
+      none
+    else
+      binSearchAux lt as k lo ⟨m - 1, by grind⟩ (by grind)
+  else
+    (some a)
+termination_by hi.1 - lo.1
+
+#print binSearchAux
+set_option pp.fieldNotation false in
+#print binSearchAux._unary
+
+def binSearch {α : Type u} (as : Array α) (k : α) (lt : α → α → Bool) : Option α :=
+  let lo := 0
+  let hi := as.size - 1
+  if h : lo < as.size then
+    binSearchAux lt as k ⟨lo, by grind⟩ ⟨hi, by grind⟩ (by grind)
   else
     none
 
-set_option trace.chako true in
-example (xs : Array Nat) (h : n ∈ xs) : xs.binSearch n Nat.blt = some n := by
+/- Lacks (h : xs.Sorted Nat.blt) -/
+theorem complete (xs : Array Nat) (h : n ∈ xs) : xs.binSearch n Nat.blt = some n := by
   chako
 
-example (xs : Array Nat) : xs.binSearch n Nat.blt = some y ↔ n = y := by
+/- Is an → not a ↔ -/
+theorem sound (xs : Array Nat) : xs.binSearch n Nat.blt = some y ↔ n = y := by
   chako
